\section{Mercredi 23 Décembre}

\begin{exercice}
    Résout les équations suivantes:
    \begin{exerciceenumnoeq}
        \item $x+3=7$
        \item $2x-5=6$
        \item $-x-3=4$
        \item $-6x+3=-9$
        \item $4(x-5) = -6$
        \item $\frac35 = \frac{x}7$
        \item $\frac{11}4 = \frac7x$
        \item $\frac43x + 6 = 10$
        \item $\frac52x - \frac32 = \frac{11}2$
        \item $\frac18x - \frac75 = \frac{13}{20}$
    \end{exerciceenumnoeq}
\end{exercice}

\begin{exercice}
    Résout les équations suivantes:
    \begin{exerciceenumnoeq}
        \item $3x+4 = 2x-1$
        \item $x+7 = 3-5x$
        \item $\frac23x + \frac43 = \frac95 - \frac73x$
        \item $9x - \frac52 = 2x+\frac56$
        \item $\frac37\left(\frac73x + 2\right) = \frac23\left(4 - \frac75x\right)$
        \item $\frac73 - 5x + \frac{16}9 = 2 - x + \frac56$
        \item $\frac{-2x-5}5 = \frac{3x-8}4$
    \end{exerciceenumnoeq}
\end{exercice}

\begin{exercice}
    Résout les équations suivantes en appliquant la méthode du produit nul.
    \begin{exerciceenumnoeq}
        \item $(5x-2)(x+6) = 0$
        \item $(3x+4)(4x+5) = 0$
        \item $(3x-5)(-9x+1) = 0$
        \item $\left(x-\frac12\right)\left(2x+\frac13\right)=0$
        \item $\left(\frac35x-1\right)\left(\frac83x+2\right) = 0$
    \end{exerciceenumnoeq}
\end{exercice}

\exequationpremierdegree{10}

\exequationproduitnul{10}